Tidy

examples/steel/AggregateRef.fst
@@ -25,6 +25,7 @@ let put_put' (l: lens 'a 'b) (s: 'a) (v w: 'b)
 (** Updating the target of a lens *)
 let lens_upd (l: lens 'a 'b) (f: 'b -> 'b) (s: 'a): 'a = l.put (f (l.get s)) s
 
+(** The identity lens *)
 let const (x: 'a) (b: 'b): 'a = x
 let lens_id #a : lens a a = {
   get = id;
@@ -34,6 +35,7 @@ let lens_id #a : lens a a = {
   put_put = (fun _ _ _ -> ());
 }
 
+(** Lens composition *)
 let get_comp (l: lens 'a 'b) (m: lens 'b 'c) (s: 'a): 'c = m.get (l.get s)
 let put_comp (l: lens 'a 'b) (m: lens 'b 'c) (v: 'c) (s: 'a): 'a =
   lens_upd l (m.put v) s
@@ -45,45 +47,6 @@ let lens_comp (l: lens 'a 'b) (m: lens 'b 'c): lens 'a 'c = {
   put_put = (fun _ _ _ -> ());
 }
 
-let refine_t (f: 'a -> prop) = x:'a{f x}
-
-let ( << ) (f: 'b -> 'c) (g: 'a -> 'b) (x: 'a): 'c = f (g x)
-let lens_refine_get (l: lens 'a 'b) f (s: refine_t (f << l.get)): refine_t f = l.get s
-let lens_refine_put (l: lens 'a 'b) f (v: refine_t f) (s: refine_t (f << l.get)): refine_t (f << l.get) =
-  l.put v s
-let lens_refine (l: lens 'a 'b) (f: 'b -> prop) : lens (refine_t (f << l.get)) (refine_t f) = {
-  get = lens_refine_get l f;
-  put = lens_refine_put l f;
-  get_put = (fun _ _ -> ());
-  put_get = (fun _ -> ());
-  put_put = (fun _ _ _ -> ());
-}
-
-let lens_fst_put (x:'a) (xy: 'a & 'b): 'a & 'b = (x, snd xy)
-let lens_fst #a #b : lens (a & b) a = {
-  get = fst;
-  put = lens_fst_put;
-  get_put = (fun _ _ -> ());
-  put_get = (fun _ -> ());
-  put_put = (fun _ _ _ -> ());
-}
-
-(** We can create lenses for unions if we know which case of the union we are in: *)
-
-let either_l a b = x:either a b{Inl? x}
-let lens_left_put (y: 'a) (x:either_l 'a 'b): either_l 'a 'b =
-  Inl y
-let lens_left #a #b : lens (either_l a b) a = {
-  get = Inl?.v;
-  put = lens_left_put;
-  get_put = (fun _ _ -> ());
-  put_get = (fun _ -> ());
-  put_put = (fun _ _ _ -> ());
-}
-
-let lens_left_fst #a #b #c: lens (either_l (a & b) c) a = lens_comp lens_left lens_fst
-let lens_fst_left #a #b #c: lens ((either_l a b) & c) a = lens_comp lens_fst lens_left
-
 (** The non-computational part of frame_preserving_upd
     TODO: move this and lemmas about this to FStar.PCM.fst *)
 let frame_pres_on (p: pcm 'a) (f: 'a -> 'a) (x y: Ghost.erased 'a)
@@ -93,7 +56,6 @@ let frame_pres_on (p: pcm 'a) (f: 'a -> 'a) (x y: Ghost.erased 'a)
   (forall (frame:'a{composable p x frame}).{:pattern composable p x frame}
      composable p y frame /\
      (op p x frame == v ==> op p y frame == f v))
-
 let frame_pres (p: pcm 'a) (f: 'a -> 'a) (x y: Ghost.erased 'a) =
   forall (v:'a{p.refine v /\ compatible p x v}).{:pattern compatible p x v}
   frame_pres_on p f x y v
@@ -117,18 +79,21 @@ let frame_pres_intro (p: pcm 'a) (f: 'a -> 'a) (x y: Ghost.erased 'a)
   let _ = g in ()
 
 (** Given PCMs (p: pcm a) and (q: pcm b), a (pcm_lens p q) is a (lens a b)
-    with the extra requirement that [get] and [put] be PCM morphisms. *)
+    with the extra requirement that get and put be PCM morphisms. *)
 noeq type pcm_lens #a #b (p: pcm a) (q: pcm b) = {
   l: lens a b;
-  get_refine: s:a -> Lemma (requires p.refine s) (ensures q.refine (l.get s)) [SMTPat (p.refine s)];
+  get_refine: s:a ->
+    Lemma (requires p.refine s) (ensures q.refine (l.get s)) [SMTPat (p.refine s)];
   get_op: s:a -> t:a ->
     Lemma
       (requires composable p s t)
       (ensures composable q (l.get s) (l.get t) /\ 
                l.get (op p s t) == op q (l.get s) (l.get t))
-               // Technically, this distributivity law is derivable from the one for put:
-               //   get (s * t) = get (put (get s) s * put (get t) t)
-               //   = get (put (get s * get t) (s * t)) = get s * get t
+               (* Technically, this distributivity law is derivable from the one for put:
+                    get (s * t)
+                    = get (put (get s) s * put (get t) t)
+                    = get (put (get s * get t) (s * t))
+                    = get s * get t *)
     [SMTPat (composable p s t); SMTPat (l.get (op p s t))];
   put_refine: s:a -> v:b ->
     Lemma (requires p.refine s /\ q.refine v) (ensures p.refine (l.put v s))
@@ -140,160 +105,69 @@ noeq type pcm_lens #a #b (p: pcm a) (q: pcm b) = {
                l.put (op q v w) (op p s t) == op p (l.put v s) (l.put w t))
     [SMTPat (l.put (op q v w) (op p s t)); SMTPat (composable p (l.put v s) (l.put w t))];
 }
+let get (#p: pcm 'a) (#q: pcm 'b) (l: pcm_lens p q) (s: 'a): 'b = l.l.get s
+let put (#p: pcm 'a) (#q: pcm 'b) (l: pcm_lens p q) (v: 'b) (s: 'a): 'a = l.l.put v s
+let upd (#p: pcm 'a) (#q: pcm 'b) (l: pcm_lens p q) (f: 'b -> 'b) (s: 'a): 'a = lens_upd l.l f s
 
 let pcm_lens_compatible_get (#p: pcm 'a) (#q: pcm 'b) (l: pcm_lens p q) (x y: 'a)
-: Lemma (requires compatible p x y) (ensures compatible q (l.l.get x) (l.l.get y))
-= compatible_elim p x y (compatible q (l.l.get x) (l.l.get y)) (fun frame_x ->
+: Lemma (requires compatible p x y) (ensures compatible q (get l x) (get l y))
+= compatible_elim p x y (compatible q (get l x) (get l y)) (fun frame_x ->
   let _ = l.get_op frame_x x in
-  compatible_intro q (l.l.get x) (l.l.get y) (l.l.get frame_x))
+  compatible_intro q (get l x) (get l y) (get l frame_x))
 
+(** The upd function of a pcm_lens lifts frame-preserving updates on the target to
+    frame-preserving updates on the source *)
 let pcm_lens_frame_pres (p: pcm 'a) (q: pcm 'b) (l: pcm_lens p q) (s: 'a) (v: 'b) (f: 'b -> 'b)
 : Lemma
-    (requires frame_pres q f (l.l.get s) v)
-    (ensures frame_pres p (lens_upd l.l f) s (l.l.put v s))
-    [SMTPat (frame_pres q f (l.l.get s) v)]
-= frame_pres_intro p (lens_upd l.l f) s (l.l.put v s) (fun full ->
-    assert (p.refine full);
-    assert (compatible p s full);
-    assert (lens_upd l.l f full == l.l.put (f (l.l.get full)) full);
+    (requires frame_pres q f (get l s) v)
+    (ensures frame_pres p (upd l f) s (put l v s))
+    [SMTPat (frame_pres q f (get l s) v)]
+= frame_pres_intro p (upd l f) s (put l v s) (fun full ->
     let _ = l.get_refine in
-    assert (q.refine (l.l.get full));
     pcm_lens_compatible_get l s full;
-    assert (compatible q (l.l.get s) (l.l.get full));
-    assert (q.refine (f (l.l.get full)));
     let _ = l.put_refine in
-    assert (p.refine (lens_upd l.l f full));
-    assert (compatible q v (f (l.l.get full)));
-    let goal = frame_pres_on p (lens_upd l.l f) s (l.l.put v s) full in
+    let goal = frame_pres_on p (upd l f) s (put l v s) full in
     compatible_elim p s full goal (fun frame_s ->
-    compatible_elim q v (f (l.l.get full)) goal (fun frame_v ->
-    assert (composable q v frame_v /\ op q frame_v v == f (l.l.get full));
-    let frame_vs: 'a = l.l.put frame_v frame_s in
+    compatible_elim q v (f (get l full)) goal (fun frame_v ->
+    let frame_vs: 'a = put l frame_v frame_s in
     l.put_op s frame_s v frame_v;
-    assert (composable p (l.l.put v s) frame_vs);
-    p.comm frame_vs (l.l.put v s);
+    p.comm frame_vs (put l v s);
     q.comm v frame_v;
     p.comm s frame_s;
-    assert (op p frame_vs (l.l.put v s) == op p (l.l.put v s) frame_vs);
-    assert (op p frame_vs (l.l.put v s) == l.l.put (op q v frame_v) (op p s frame_s));
-    assert (op p frame_vs (l.l.put v s) == l.l.put (op q v frame_v) (op p s frame_s));
-    assert (op p frame_vs (l.l.put v s) == lens_upd l.l f full);
-    compatible_intro p (l.l.put v s) (lens_upd l.l f full) frame_vs;
+    compatible_intro p (put l v s) (upd l f full) frame_vs;
     let aux (frame:'a{composable p s frame})
-    : Lemma (composable p (l.l.put v s) frame /\
-             (op p s frame == full ==> op p (l.l.put v s) frame == lens_upd l.l f full))
+    : Lemma (composable p (put l v s) frame /\
+             (op p s frame == full ==> op p (put l v s) frame == upd l f full))
     = l.get_op s frame;
-      assert (composable q (l.l.get s) (l.l.get frame));
-      assert (composable q v (l.l.get frame));
-      assert (composable p s frame);
-      l.put_op s frame v (l.l.get frame);
-      let aux ()
-      : Lemma (requires op p s frame == full) 
-              (ensures op p (l.l.put v s) frame == lens_upd l.l f full)
-      = assert (composable p (l.l.put v s) (l.l.put (l.l.get frame) frame));
-        assert (op p (l.l.put v s) frame == op p (l.l.put v s) (l.l.put (l.l.get frame) frame));
-        assert (op p (l.l.put v s) frame == l.l.put (op q v (l.l.get frame)) (op p s frame));
-        assert (op p (l.l.put v s) frame == l.l.put (op q v (l.l.get frame)) full);
-        ()
-      in ()
+      l.put_op s frame v (get l frame)
     in FStar.Classical.forall_intro aux)))
 
-// let pcm_lens_id (#p: pcm 'a): pcm_lens p p
-//   = {raw = lens_id; upd_resp_pcm = (fun _ _ _ -> ())}
-// let pcm_lens_comp (#p: pcm 'a) (#q: pcm 'b) (#r: pcm 'c)
-//   (l: pcm_lens p q) (m: pcm_lens q r): pcm_lens p r
-//   = {raw = lens_comp l.raw m.raw; upd_resp_pcm = (fun _ _ _ -> ())}
-// 
-// let get (#p: pcm 'a) (#q: pcm 'b) (l: pcm_lens p q) (s: 'a): 'b = l.raw.get s
-// let put (#p: pcm 'a) (#q: pcm 'b) (l: pcm_lens p q) (v: 'b) (s: 'a): 'a = l.raw.put v s
-// let upd (#p: pcm 'a) (#q: pcm 'b) (l: pcm_lens p q) (f: 'b -> 'b) (s: 'a): 'a = lens_upd l.raw f s
-
-open Aggregates
-
-// let pcm_lens_fst #a #b (p: pcm a) (q: pcm b): pcm_lens (tuple_pcm p q) p = {
-//   l = lens_fst;
-//   upd_resp_pcm = (fun (x, y) x' f ->
-//     assert (forall (v:a{p.refine v /\ compatible p x v}). p.refine (f v) /\ compatible p x' (f v));
-//     frame_pres_intro (tuple_pcm p q) (lens_upd lens_fst f) (x, y) (x', y)
-//       (fun (v, w) ->
-//         let compat_ty = compatible (tuple_pcm p q) (x', y) (f v, w) in
-//         compatible_elim p x' (f v) compat_ty (fun frame_v ->
-//         compatible_elim q y w compat_ty (fun frame_w ->
-//         compatible_intro (tuple_pcm p q) (x', y) (f v, w) (frame_v, frame_w)))));
-// }
-
-(** A PCM for binary sums *)
-
-let either_composable (p: pcm 'a) (q: pcm 'b): symrel (option (either 'a 'b)) =
-  fun x y -> match x, y with
-    | None, _ | _, None -> True
-    | Some (Inl x), Some (Inl y) -> composable p x y
-    | Some (Inr x), Some (Inr y) -> composable q x y
-    | _, _ -> False
-let either_op (p: pcm 'a) (q: pcm 'b) (x: option (either 'a 'b))
-  (y: option (either 'a 'b){either_composable p q x y})
-: option (either 'a 'b) = match x, y with
-  | None, z | z, None -> z
-  | Some (Inl x), Some (Inl y) -> Some (Inl (op p x y))
-  | Some (Inr x), Some (Inr y) -> Some (Inr (op q x y))
-    
-let either_pcm (p: pcm 'a) (q: pcm 'b): pcm (option (either 'a 'b)) = {
-  p = {composable = either_composable p q; op = either_op p q; one = None};
-  comm = (fun x y -> match x, y with
-    | None, _ | _, None -> ()
-    | Some (Inl x), Some (Inl y) -> p.comm x y
-    | Some (Inr x), Some (Inr y) -> q.comm x y);
-  assoc = (fun x y z -> match x, y, z with
-    | Some (Inl x), Some (Inl y), Some (Inl z) -> p.assoc x y z
-    | Some (Inr x), Some (Inr y), Some (Inr z) -> q.assoc x y z
-    | _, _, _ -> ());
-  assoc_r = (fun x y z -> match x, y, z with
-    | Some (Inl x), Some (Inl y), Some (Inl z) -> p.assoc_r x y z
-    | Some (Inr x), Some (Inr y), Some (Inr z) -> q.assoc_r x y z
-    | _, _, _ -> ());
-  is_unit = (fun x -> ());
-  refine = (fun x -> match x with
-    | None -> True
-    | Some (Inl x) -> p.refine x
-    | Some (Inr x) -> q.refine x);
+(** The identity lens is a pcm_lens *)
+let pcm_lens_id (#p: pcm 'a): pcm_lens p p = {
+  l = lens_id; 
+  get_refine = (fun _ -> ());
+  get_op = (fun _ _ -> ());
+  put_refine = (fun _ _ -> ());
+  put_op = (fun _ _ _ _ -> ());
 }
 
-(** A PCM for possibly uninitialized data *)
-
-type init a =
-| Uninitialized : init a
-| One : init a
-| Initialized : a -> init a
-
-let init_comp (p: pcm 'a): symrel (init 'a) = fun x y -> match x, y with
-  | One, _ | _, One -> True
-  | Uninitialized, Uninitialized -> True
-  | Initialized x, Initialized y -> composable p x y
-  | _, _ -> False
-
-let init_op (p: pcm 'a) (x: init 'a) (y: init 'a{init_comp p x y}): init 'a = match x, y with
-  | One, z | z, One -> z
-  | Uninitialized, Uninitialized -> Uninitialized
-  | Initialized x, Initialized y -> Initialized (op p x y)
-
-let init_pcm (p: pcm 'a): pcm (init 'a) = {
-  p = {composable = init_comp p; op = init_op p; one = One #'a};
-  comm = (fun x y -> match x, y with
-    | Initialized x, Initialized y -> p.comm x y
-    | _, _ -> ());
-  assoc = (fun x y z -> match x, y, z with
-    | Initialized x, Initialized y, Initialized z -> p.assoc x y z
-    | _, _, _ -> ());
-  assoc_r = (fun x y z -> match x, y, z with
-    | Initialized x, Initialized y, Initialized z -> p.assoc_r x y z
-    | _, _, _ -> ());
-  is_unit = (fun _ -> ());
-  refine = (fun x -> match x with
-    | Initialized x -> p.refine x
-    | _ -> True)
+(** pcm_lens composition is lens composition *)
+let pcm_lens_comp (#p: pcm 'a) (#q: pcm 'b) (#r: pcm 'c)
+  (l: pcm_lens p q) (m: pcm_lens q r): pcm_lens p r = 
+{
+  l = lens_comp l.l m.l;
+  get_refine = (fun _ -> let _ = l.get_refine in let _ = m.get_refine in ());
+  get_op = (fun s t -> l.get_op s t; m.get_op (get l s) (get l t));
+  put_refine = (fun s v -> let _ = l.put_refine in let _ = m.put_refine in let _ = l.get_refine in ());
+  put_op = (fun s t v w ->
+    l.get_op s t;
+    m.put_op (get l s) (get l t) v w;
+    l.put_op s t (put m v (get l s)) (put m w (get l t)))
 }
 
 (** A refinement of a PCM p *)
+
+let refine_t (f: 'a -> prop) = x:'a{f x}
 
 noeq type pcm_refinement #a (p: pcm a) = {
   f: a -> prop;
@@ -324,25 +198,143 @@ let trivial_refinement (p: pcm 'a): pcm_refinement p = {
   new_one_is_refined_unit = p.is_unit;
 }
 
-let inl_refinement (p: pcm 'a) (q: pcm 'b): pcm_refinement (either_pcm p q) = {
-  f = (fun (x: option (either 'a 'b)) -> Some? x /\ Inl? (Some?.v x));
-  f_closed_under_op = (fun _ _ -> ());
-  new_one = Some (Inl #_ #'b p.p.one);
-  new_one_is_refined_unit = (fun (Some (Inl x)) -> p.is_unit x);
-}
-
 (** A ref is a pcm_lens combined with a Steel.Memory.ref for the base type 'a.
     The base type of the lens, unlike the Steel.Memory.ref, is refined by a refinement re. *)
 noeq type ref (a: Type u#a) (b: Type u#b) = {
   p: pcm a;
   re: pcm_refinement p;
   q: pcm b;
-  l: pcm_lens (pcm_refine p re) q;
+  pl: pcm_lens (pcm_refine p re) q;
   r: M.ref a p;
 }
 
-// (** A ref r points to a value v if r `Steel.Memory.pts_to` put v one, where
-//     - put comes from r's pcm_lens
-//     - one is the unit of r's refined PCM for the source type *)
-// let pts_to (r: ref 'a 'b) (v: 'b): M.slprop =
-//   M.pts_to r.r (put r.l v (pcm_refine r.p r.re).P.p.one)
+(** A ref r points to a value v if r `Steel.Memory.pts_to` put v one, where
+    - put comes from r's pcm_lens
+    - one is the unit of r's refined PCM for the source type *)
+let pts_to (r: ref 'a 'b) (v: 'b): M.slprop =
+  M.pts_to r.r (put r.pl v (pcm_refine r.p r.re).P.p.one)
+
+(*
+
+TODO:
+- Lens for a field of a prod_pcm
+- Refinement for a case of a union_pcm
+- Lens (with corresponding refinement) for a case of a union_pcm
+- Types of basic Steel operations manipulating pts_to
+
+*)
+
+(** Basic lenses *)
+
+open Aggregates
+
+let lens_fst_put (x:'a) (xy: 'a & 'b): 'a & 'b = (x, snd xy)
+let lens_fst #a #b : lens (a & b) a = {
+  get = fst;
+  put = lens_fst_put;
+  get_put = (fun _ _ -> ());
+  put_get = (fun _ -> ());
+  put_put = (fun _ _ _ -> ());
+}
+
+let pcm_lens_fst #a #b (p: pcm a) (q: pcm b): pcm_lens (tuple_pcm p q) p = {
+  l = lens_fst;
+  get_refine = (fun _ -> ());
+  get_op = (fun _ _ -> ());
+  put_refine = (fun _ _ -> ());
+  put_op = (fun _ _ _ _ -> ());
+}
+
+(** We can create lenses for unions if we know which case of the union we are in: *)
+
+let either_l a b = x:either a b{Inl? x}
+let lens_left_put (y: 'a) (x:either_l 'a 'b): either_l 'a 'b =
+  Inl y
+let lens_left #a #b : lens (either_l a b) a = {
+  get = Inl?.v;
+  put = lens_left_put;
+  get_put = (fun _ _ -> ());
+  put_get = (fun _ -> ());
+  put_put = (fun _ _ _ -> ());
+}
+
+let lens_left_fst #a #b #c: lens (either_l (a & b) c) a = lens_comp lens_left lens_fst
+let lens_fst_left #a #b #c: lens ((either_l a b) & c) a = lens_comp lens_fst lens_left
+
+(** A PCM for binary sums *)
+
+let either_composable (p: pcm 'a) (q: pcm 'b): symrel (option (either 'a 'b)) =
+  fun x y -> match x, y with
+    | None, _ | _, None -> True
+    | Some (Inl x), Some (Inl y) -> composable p x y
+    | Some (Inr x), Some (Inr y) -> composable q x y
+    | _, _ -> False
+let either_op (p: pcm 'a) (q: pcm 'b) (x: option (either 'a 'b))
+  (y: option (either 'a 'b){either_composable p q x y})
+: option (either 'a 'b) = match x, y with
+  | None, z | z, None -> z
+  | Some (Inl x), Some (Inl y) -> Some (Inl (op p x y))
+  | Some (Inr x), Some (Inr y) -> Some (Inr (op q x y))
+    
+let either_pcm (p: pcm 'a) (q: pcm 'b): pcm (option (either 'a 'b)) = P.({
+  p = {composable = either_composable p q; op = either_op p q; one = None};
+  comm = (fun x y -> match x, y with
+    | None, _ | _, None -> ()
+    | Some (Inl x), Some (Inl y) -> p.comm x y
+    | Some (Inr x), Some (Inr y) -> q.comm x y);
+  assoc = (fun x y z -> match x, y, z with
+    | Some (Inl x), Some (Inl y), Some (Inl z) -> p.assoc x y z
+    | Some (Inr x), Some (Inr y), Some (Inr z) -> q.assoc x y z
+    | _, _, _ -> ());
+  assoc_r = (fun x y z -> match x, y, z with
+    | Some (Inl x), Some (Inl y), Some (Inl z) -> p.assoc_r x y z
+    | Some (Inr x), Some (Inr y), Some (Inr z) -> q.assoc_r x y z
+    | _, _, _ -> ());
+  is_unit = (fun x -> ());
+  refine = (fun x -> match x with
+    | None -> True
+    | Some (Inl x) -> p.refine x
+    | Some (Inr x) -> q.refine x);
+})
+
+let inl_refinement (p: pcm 'a) (q: pcm 'b): pcm_refinement (either_pcm p q) = {
+  f = (fun (x: option (either 'a 'b)) -> Some? x /\ Inl? (Some?.v x));
+  f_closed_under_op = (fun _ _ -> ());
+  new_one = Some (Inl #_ #'b p.P.p.one);
+  new_one_is_refined_unit = (fun (Some (Inl x)) -> p.is_unit x);
+}
+
+(** A PCM for possibly uninitialized data *)
+
+type init a =
+| Uninitialized : init a
+| One : init a
+| Initialized : a -> init a
+
+let init_comp (p: pcm 'a): symrel (init 'a) = fun x y -> match x, y with
+  | One, _ | _, One -> True
+  | Uninitialized, Uninitialized -> True
+  | Initialized x, Initialized y -> composable p x y
+  | _, _ -> False
+
+let init_op (p: pcm 'a) (x: init 'a) (y: init 'a{init_comp p x y}): init 'a = match x, y with
+  | One, z | z, One -> z
+  | Uninitialized, Uninitialized -> Uninitialized
+  | Initialized x, Initialized y -> Initialized (op p x y)
+
+let init_pcm (p: pcm 'a): pcm (init 'a) = P.({
+  p = {composable = init_comp p; op = init_op p; one = One #'a};
+  comm = (fun x y -> match x, y with
+    | Initialized x, Initialized y -> p.comm x y
+    | _, _ -> ());
+  assoc = (fun x y z -> match x, y, z with
+    | Initialized x, Initialized y, Initialized z -> p.assoc x y z
+    | _, _, _ -> ());
+  assoc_r = (fun x y z -> match x, y, z with
+    | Initialized x, Initialized y, Initialized z -> p.assoc_r x y z
+    | _, _, _ -> ());
+  is_unit = (fun _ -> ());
+  refine = (fun x -> match x with
+    | Initialized x -> p.refine x
+    | _ -> True)
+})
